src3.0/Transforms/phiplacement_bsim_wfS.v
@@ -8,28 +8,498 @@ Require Import primitives.
 Require Import mem2reg.
 Require Import opsem_props.
 Require Import palloca_props.
-Require Import program_sim.
+Require Import phiplacement_bsim_defs.
 Require Import top_wfS.
 
-Lemma phinodes_placement_wf_fdef: forall los nts Ps1 f rd pid ty al Ps2
-  (HwfF: wf_fdef [module_intro los nts (Ps1 ++ product_fdef f :: Ps2)]
-           (module_intro los nts (Ps1 ++ product_fdef f :: Ps2)) f),
-  wf_fdef [module_intro los nts (Ps1 ++ product_fdef f :: Ps2)]
-    (module_intro los nts (Ps1 ++ product_fdef f :: Ps2))
-    (phinodes_placement f rd pid ty al (successors f)
-       (make_predecessors (successors f))).
+(*********************************************************)
+(*
+   preserving reachablity and succ does not require WF_PhiInfo 
+   So, we do not use PhiInfo 
+*)
+
+Definition phinodes_placement_fdef pid ty al nids sccs prds (f:fdef): fdef :=
+match f with
+| fdef_intro fh bs => 
+  fdef_intro fh (List.map (phinodes_placement_block pid ty al nids sccs prds) bs)
+end.
+
+Lemma phinodes_placement_fdef_spec1: forall rd pid ty al sccs prds f,
+  phinodes_placement rd pid ty al sccs prds f  =
+  phinodes_placement_fdef pid ty al 
+    (fst (gen_fresh_ids rd (getFdefLocs f))) sccs prds f.
+Proof.
+  unfold phinodes_placement, phinodes_placement_fdef.
+  intros.
+  destruct_let. destruct f. auto.
+Qed.
+
+Lemma phinodes_placement_block__getBlockLabel: forall pid t al nids succs
+  preds b,
+  getBlockLabel b =
+  getBlockLabel (phinodes_placement_block pid t al nids succs preds b).
+Proof.
+  destruct b as [l0 ? ? ?]; simpl.
+    destruct (nids ! l0) as [[[]]|]; auto.
+    destruct (preds ! l0) as [[]|]; auto.
+Qed.
+
+Lemma phinodes_placement_block__getBlockTmn: forall pid t al nids succs preds b, 
+  getBlockTmn b = 
+    getBlockTmn (phinodes_placement_block pid t al nids succs preds b).
+Proof. 
+  destruct b as [l0 ? ? t0]; simpl.
+    destruct (nids ! l0) as [[[]]|]; auto.
+    destruct (preds ! l0) as [[]|]; auto.
+Qed.
+
+Lemma phinodes_placement_block__getBlockTmn_match: forall pid t al nids succs 
+  preds b, 
+  terminator_match (getBlockTmn b) 
+    (getBlockTmn (phinodes_placement_block pid t al nids succs preds b)).
+Proof. 
+  intros.
+  rewrite <- phinodes_placement_block__getBlockTmn.
+  destruct (getBlockTmn b); simpl; auto.
+Qed.
+
+Lemma phinodes_placement_fdef_spec2: forall pid t al nids succs preds fh bs, 
+  phinodes_placement_fdef pid t al nids succs preds (fdef_intro fh bs) = 
+    fdef_intro fh 
+      (List.map (phinodes_placement_block pid t al nids succs preds) bs).
+Proof. simpl. auto. Qed.
+
+Definition phiplacement pid t al nids succs preds := mkPass 
+(phinodes_placement_block pid t al nids succs preds)
+(phinodes_placement_fdef pid t al nids succs preds)
+(phinodes_placement_fdef_spec2 pid t al nids succs preds)
+(phinodes_placement_block__getBlockLabel pid t al nids succs preds)
+(phinodes_placement_block__getBlockTmn_match pid t al nids succs preds)
+.
+
+Ltac fold_phiplacement_tac :=
+  match goal with
+  | |- context [phinodes_placement_fdef ?pid ?t ?al ?nids ?succs ?preds ?f] =>
+    replace (phinodes_placement_fdef pid t al nids succs preds f) 
+      with (ftrans (phiplacement pid t al nids succs preds) f); auto
+  end.
+
+Lemma phinodes_placement_reachablity_analysis: forall f rd pid ty al,
+  reachablity_analysis f =
+  reachablity_analysis
+     (phinodes_placement rd pid ty al (successors f)
+        (make_predecessors (successors f)) f).
+Proof.
+  intros.
+  rewrite phinodes_placement_fdef_spec1.
+  fold_phiplacement_tac.
+  apply TransCFG.pres_reachablity_analysis.
+Qed.
+
+Lemma phinodes_placement_successors: forall f rd pid ty al,
+  successors f =
+  successors
+    (phinodes_placement rd pid ty al (successors f)
+       (make_predecessors (successors f)) f).
+Proof.
+  intros.
+  rewrite phinodes_placement_fdef_spec1.
+  fold_phiplacement_tac.
+  apply TransCFG.pres_successors.
+Qed.
+
+(* preserving uniqness and wfness require WF_PhiInfo *)
+
+Definition phinodes_placement_blk (pinfo:PhiInfo) (b:block): block :=
+phinodes_placement_block (PI_id pinfo) (PI_typ pinfo) (PI_align pinfo)
+  (PI_newids pinfo) (PI_succs pinfo) (PI_preds pinfo) b.
+
+Definition phinodes_placement_f (pinfo:PhiInfo) (f:fdef): fdef :=
+match f with
+| fdef_intro fh bs => fdef_intro fh (List.map (phinodes_placement_blk pinfo) bs)
+end.
+
+Lemma phinodes_placement_f_spec1: forall pinfo,
+  phinodes_placement (PI_rd pinfo) (PI_id pinfo) (PI_typ pinfo) (PI_align pinfo)
+    (PI_succs pinfo) (PI_preds pinfo) (PI_f pinfo) =
+  phinodes_placement_f pinfo (PI_f pinfo).
+Proof.
+  unfold phinodes_placement, phinodes_placement_f, phinodes_placement_blk, 
+         PI_newids.
+  intros.
+  destruct_let. destruct (PI_f pinfo). auto.
+Qed.
+
+Lemma phinodes_placement_blk__getBlockLabel: forall pinfo b,
+  getBlockLabel b =
+  getBlockLabel (phinodes_placement_blk pinfo b).
+Proof.
+  unfold phinodes_placement_blk. intro.
+  apply phinodes_placement_block__getBlockLabel; auto.
+Qed.
+
+Lemma phinodes_placement_blk__getBlockTmn_match: forall pinfo b, 
+  terminator_match (getBlockTmn b) 
+    (getBlockTmn (phinodes_placement_blk pinfo b)).
+Proof. 
+  intros.
+  unfold phinodes_placement_blk.
+  apply phinodes_placement_block__getBlockTmn_match; auto.
+Qed.
+
+Lemma phinodes_placement_f_spec2: forall pinfo fh bs, 
+  phinodes_placement_f pinfo (fdef_intro fh bs) = 
+    fdef_intro fh (List.map (phinodes_placement_blk pinfo) bs).
+Proof. simpl. auto. Qed.
+
+Definition PhiPlacement pinfo := mkPass 
+(phinodes_placement_blk pinfo)
+(phinodes_placement_f pinfo)
+(phinodes_placement_f_spec2 pinfo)
+(phinodes_placement_blk__getBlockLabel pinfo)
+(phinodes_placement_blk__getBlockTmn_match pinfo)
+.
+
+Ltac fold_PhiPlacement_tac :=
+repeat match goal with
+| |- context [phinodes_placement_f ?pinfo ?f] =>
+  replace (phinodes_placement_f pinfo f) 
+    with (ftrans (PhiPlacement pinfo) f); auto
+| |- context [phinodes_placement_blk ?pinfo ?b] =>
+  replace (phinodes_placement_blk pinfo b) 
+    with (btrans (PhiPlacement pinfo) b); auto
+| |- context [phinodes_placement_f ?pinfo] =>
+  replace (phinodes_placement_f pinfo) 
+    with (ftrans (PhiPlacement pinfo)); auto
+| |- context [phinodes_placement_blk ?pinfo] =>
+  replace (phinodes_placement_blk pinfo) 
+    with (btrans (PhiPlacement pinfo)); auto
+end.
+
+Ltac unfold_PhiPlacement_tac :=
+repeat match goal with
+| |- context [ftrans (PhiPlacement ?pinfo) ?f] =>
+  replace (ftrans (PhiPlacement pinfo) f)
+    with (phinodes_placement_f pinfo f); auto
+| |- context [btrans (PhiPlacement ?pinfo) ?b] =>
+  replace (btrans (PhiPlacement pinfo) b)
+    with (phinodes_placement_blk pinfo b); auto
+| |- context [ftrans (PhiPlacement ?pinfo)] =>
+  replace (ftrans (PhiPlacement pinfo))
+    with (phinodes_placement_f pinfo); auto
+| |- context [btrans (PhiPlacement ?pinfo)] =>
+  replace (btrans (PhiPlacement pinfo))
+    with (phinodes_placement_blk pinfo); auto
+end.
+
+(*********************************************************)
+(* wfness *)
+
+Lemma wf_typ_independent: forall (sys1 sys2 : system) (td: targetdata)
+  (t: typ) (Hwft: wf_typ sys1 td t), wf_typ sys2 td t.
+Proof.
+  intros.
+  inv Hwft.
+  constructor; eauto using wf_styp_independent, noncycled_independent.
+Qed.
+
+Lemma uniqF__uniqBlocksLocs : forall fh lb,
+  uniqFdef (fdef_intro fh lb) -> NoDup (getBlocksLocs lb).
+Proof.
+  intros. destruct fh. inversion H. split_NoDup; auto.
+Qed.
+
+Section PresWF.
+
+Variable (los:layouts) (nts:namedts) (Ps1 Ps2:products) (pinfo:PhiInfo).
+Hypothesis (Hwfpi: WF_PhiInfo pinfo).
+
+Lemma phinodes_placement_wf_insn : forall (M M':module) (f':fdef)
+  (HeqM: M = module_intro los nts (Ps1 ++ product_fdef (PI_f pinfo) :: Ps2))
+  (HeqM': M' = module_intro los nts (Ps1 ++ product_fdef f' :: Ps2))
+  (HeqF': f' = phinodes_placement_f pinfo (PI_f pinfo)) b b' 
+  (Heqb': b' = phinodes_placement_blk pinfo b) instr
+  (HwfI : wf_insn [M] M (PI_f pinfo) b instr),
+  wf_insn [M'] M' f' b' instr.
+Proof.
 Admitted.
 
-Lemma phinodes_placement_uniqFdef: forall f rd pid ty al (Huniq: uniqFdef f),
-  uniqFdef (phinodes_placement f rd pid ty al (successors f)
-             (make_predecessors (successors f))).
+Lemma phinodes_placement_wf_cmds : forall (M M':module) (f':fdef)
+  (HeqM: M = module_intro los nts (Ps1 ++ product_fdef (PI_f pinfo) :: Ps2))
+  (HeqM': M' = module_intro los nts (Ps1 ++ product_fdef f' :: Ps2))
+  (HeqF': f' = phinodes_placement_f pinfo (PI_f pinfo)) b b' 
+  (Heqb': b' = phinodes_placement_blk pinfo b) cs 
+  (Hwfcs : wf_cmds [M] M (PI_f pinfo) b cs),
+  wf_cmds [M'] M' f' b' cs.
+Proof.
 Admitted.
 
-Lemma phinodes_placement_fheaderOfFdef: forall f rd pid ty al,
-  fheaderOfFdef f =
-  fheaderOfFdef (phinodes_placement f rd pid ty al (successors f)
-                  (make_predecessors (successors f))).
+Lemma phinodes_placement_wf_phinodes : forall (M M':module) (f':fdef)
+  (HeqM: M = module_intro los nts (Ps1 ++ product_fdef (PI_f pinfo) :: Ps2))
+  (HeqM': M' = module_intro los nts (Ps1 ++ product_fdef f' :: Ps2))
+  (HeqF': f' = phinodes_placement_f pinfo (PI_f pinfo)) b b' 
+  (Heqb': b' = phinodes_placement_blk pinfo b) ps
+  (Hwfps : wf_phinodes [M] M (PI_f pinfo) b ps),
+  wf_phinodes [M'] M' f' b' ps.
+Proof.
 Admitted.
+
+Lemma phinodes_placement_lookupTypViaIDFromFdef: forall (f':fdef)
+  (HeqF': f' = phinodes_placement_f pinfo (PI_f pinfo)) id0 t
+  (Hlkty: lookupTypViaIDFromFdef (PI_f pinfo) id0 = Some t),
+  lookupTypViaIDFromFdef f' id0 = Some t.
+Admitted.
+
+Lemma phinodes_placement_wf_value : forall (M M':module) (f':fdef)
+  (HeqM: M = module_intro los nts (Ps1 ++ product_fdef (PI_f pinfo) :: Ps2))
+  (HeqM': M' = module_intro los nts (Ps1 ++ product_fdef f' :: Ps2))
+  (HeqF': f' = phinodes_placement_f pinfo (PI_f pinfo)) v t
+  (Hwfv: wf_value [M] M (PI_f pinfo) v t),
+  wf_value [M'] M' f' v t.
+Proof.
+  intros.
+  inv Hwfv; try constructor.
+(*    apply insert_lookupIDFromFdef; auto. *)
+Admitted.
+
+Lemma wf_inserted: forall (M M':module) (f':fdef) 
+  (HwfF: wf_fdef [M] M (PI_f pinfo))
+  (HeqM: M = module_intro los nts (Ps1 ++ product_fdef (PI_f pinfo) :: Ps2))
+  (HeqM': M' = module_intro los nts (Ps1 ++ product_fdef f' :: Ps2))
+  (HeqF': f' = phinodes_placement_f pinfo (PI_f pinfo)) b b' 
+  (Heqb': b' = phinodes_placement_blk pinfo b)
+  (HBinF: blockInFdefB b (PI_f pinfo) = true),
+  match (PI_newids pinfo) ! (getBlockLabel b) with
+  | Some (lid, pid, sid) =>
+      match (PI_succs pinfo) ! (getBlockLabel b) with
+      | Some (_::_) =>
+          wf_insn [M'] M' f' b' 
+            (insn_cmd (insn_load lid (PI_typ pinfo) (value_id (PI_id pinfo))
+                                 (PI_align pinfo)))
+      | _ => True
+      end /\
+      match (PI_preds pinfo) ! (getBlockLabel b) with
+      | Some ((_::_) as pds) =>
+         wf_insn [M'] M' f' b' 
+           (insn_cmd (insn_store sid (PI_typ pinfo) (value_id pid)
+                        (value_id (PI_id pinfo)) (PI_align pinfo))) /\
+         wf_phinodes [M'] M' f' b' 
+            [gen_phinode pid (PI_typ pinfo) (PI_newids pinfo) pds]
+      | _ => True
+      end
+  | _ => True
+  end.
+Proof.
+  intros. 
+  assert (wf_value [M'] M' f' (value_id (PI_id pinfo)) 
+            (typ_pointer (PI_typ pinfo))) as Hwfv.
+    admit.
+  assert (wf_typ [M'] (los,nts) (PI_typ pinfo)) as Hwft.
+    admit.
+  subst.
+  remember ((PI_newids pinfo) ! (getBlockLabel b)) as R1.
+  remember ((PI_succs pinfo) ! (getBlockLabel b)) as R2.
+  remember ((PI_preds pinfo) ! (getBlockLabel b)) as R3.
+  destruct R1 as [[[lid pid] sid]|]; auto.
+  split.
+    destruct R2 as [[]|]; auto.
+    constructor; auto.
+      admit.
+
+    destruct R3 as [[]|]; auto.
+    split.
+      constructor; auto.
+        admit.
+        admit.
+
+      constructor; auto.
+        unfold gen_phinode.
+        admit.
+
+        constructor.
+Qed.
+
+Lemma phinodes_placement_blockInSystemModuleFdefB: forall (M M':module) (f':fdef)
+  (HeqM: M = module_intro los nts (Ps1 ++ product_fdef (PI_f pinfo) :: Ps2))
+  (HeqM': M' = module_intro los nts (Ps1 ++ product_fdef f' :: Ps2))
+  (HeqF': f' = phinodes_placement_f pinfo (PI_f pinfo)) b b' 
+  (Heqb': b' = phinodes_placement_blk pinfo b)
+  (Hin: blockInSystemModuleFdefB b [M] M (PI_f pinfo)),
+  blockInSystemModuleFdefB b' [M'] M' f'.
+Admitted.
+
+Ltac inv_wf_block H :=
+let S5 := fresh "S5" in
+let M5 := fresh "M5" in
+let F5 := fresh "F5" in
+let l5 := fresh "l5" in 
+let ps5 := fresh "ps5" in 
+let cs5 := fresh "cs5" in 
+let tmn5 := fresh "tmn5" in 
+let HBinSMF := fresh "HBinSMF" in 
+let Hwfps := fresh "Hwfps" in 
+let Hwfcs := fresh "Hwfcs" in 
+let Hwfi := fresh "Hwfi" in 
+let EQ1 := fresh "EQ1" in
+let EQ2 := fresh "EQ2" in
+let EQ3 := fresh "EQ3" in 
+let EQ4 := fresh "EQ4" in
+inversion H as 
+  [S5 M5 F5 l5 ps5 cs5 tmn5 HBinSMF Hwfps Hwfcs Hwfi EQ1 EQ2 EQ3 EQ4]; subst.
+
+Lemma wf_cmds_intro: forall s m f b cs,
+  (forall c, In c cs -> wf_insn s m f b (insn_cmd c)) ->
+  wf_cmds s m f b cs.
+Proof.
+  induction cs; intros.
+    constructor.
+    constructor.
+      apply H; simpl; auto.
+      apply IHcs. intros. apply H; simpl; auto.
+Qed.
+
+Lemma wf_cmds_elim: forall s m f b cs,
+  wf_cmds s m f b cs -> forall c, In c cs -> wf_insn s m f b (insn_cmd c).
+Proof.
+  intros s m f b cs J.
+  induction J; intros.
+    inv H.
+
+    simpl in H0.
+    destruct H0 as [H0 | H0]; subst; auto.
+Qed.
+
+Lemma wf_cmds_app: forall s m f b cs2 (Hwfcs2: wf_cmds s m f b cs2) cs1
+  (Hwfcs1: wf_cmds s m f b cs1), wf_cmds s m f b (cs1++cs2).
+Proof.
+  induction cs1; simpl; intros; auto.
+    inv Hwfcs1. constructor; auto.
+Qed.
+
+Lemma wf_phinodes_app: forall s m f b ps2 (Hwfps2: wf_phinodes s m f b ps2) ps1
+  (Hwfps1: wf_phinodes s m f b ps1), wf_phinodes s m f b (ps1++ps2).
+Proof.
+  induction ps1; simpl; intros; auto.
+    inv Hwfps1. constructor; auto.
+Qed.
+
+Lemma phinodes_placement_wf_block : forall (M M':module) (f':fdef)
+  (HwfF: wf_fdef [M] M (PI_f pinfo))
+  (HeqM: M = module_intro los nts (Ps1 ++ product_fdef (PI_f pinfo) :: Ps2))
+  (HeqM': M' = module_intro los nts (Ps1 ++ product_fdef f' :: Ps2))
+  (HeqF': f' = phinodes_placement_f pinfo (PI_f pinfo)) b
+  (HwfB : wf_block [M] M (PI_f pinfo) b) (Huniq : NoDup (getBlockLocs b))
+  (HBinF: blockInFdefB b (PI_f pinfo) = true),
+  wf_block [M'] M' f' (phinodes_placement_blk pinfo b).
+Proof.
+
+Ltac phinodes_placement_wf_block_tac1 :=
+  match goal with
+  | |- wf_cmds _ _ _ _ (_++_) =>
+       apply wf_cmds_app; try solve [auto | phinodes_placement_wf_block_tac1]
+  | |- wf_cmds _ _ _ _ [_] =>
+       apply wf_cmds_cons; try solve [tauto | constructor]
+  | |- wf_phinodes _ _ _ _ (_++_) =>
+       apply wf_phinodes_app; try solve [auto | phinodes_placement_wf_block_tac1]
+  | |- wf_phinodes _ _ _ _ [_] =>
+       tauto
+  end.
+
+Ltac phinodes_placement_wf_block_tac2 :=
+  constructor; try solve [auto | phinodes_placement_wf_block_tac1].
+
+  intros.
+  assert (HwfNew:=HwfF).
+  eapply wf_inserted in HwfNew; eauto.
+  inv_wf_block HwfB. simpl in HwfNew.
+  eapply phinodes_placement_blockInSystemModuleFdefB in HBinSMF; eauto.
+  eapply phinodes_placement_wf_cmds in Hwfcs; eauto.
+  eapply phinodes_placement_wf_phinodes in Hwfps; eauto.
+  eapply phinodes_placement_wf_insn in Hwfi; eauto.
+  unfold phinodes_placement_blk, phinodes_placement_block in *.
+  remember (PI_newids pinfo) ! l5 as R1.
+  destruct R1 as [[[lid pid] sid]|]; try solve [constructor; auto].
+  remember ((PI_preds pinfo) ! l5) as R2.
+  remember ((PI_succs pinfo) ! l5) as R3.
+  destruct R2 as [[]|];
+    destruct R3 as [[]|]; 
+      try solve [simpl_env in *; phinodes_placement_wf_block_tac2].
+Qed.
+
+Lemma phinodes_placement_wf_blocks : forall (M M':module) (f':fdef)
+  (HwfF: wf_fdef [M] M (PI_f pinfo)) 
+  (HeqM: M = module_intro los nts (Ps1 ++ product_fdef (PI_f pinfo) :: Ps2))
+  (HeqM': M' = module_intro los nts (Ps1 ++ product_fdef f' :: Ps2))
+  (HeqF': f' = phinodes_placement_f pinfo (PI_f pinfo))
+  bs (Hin: forall b, In b bs -> blockInFdefB b (PI_f pinfo) = true)
+  (HwfBs : wf_blocks [M] M (PI_f pinfo) bs) (Huniq : NoDup (getBlocksLocs bs)),
+  wf_blocks [M'] M' f' (List.map (phinodes_placement_blk pinfo) bs).
+Proof.
+  intros. subst.
+  induction bs; simpl.
+    constructor.
+
+    simpl in Huniq.
+    split_NoDup. inv HwfBs.
+    constructor; auto.
+      eapply phinodes_placement_wf_block; eauto 1.
+        apply Hin; simpl; auto.
+      apply IHbs; auto.
+        intros b Hin'. apply Hin. simpl; auto.
+Qed.
+
+Lemma In_InBlocksB: forall b bs, In b bs -> InBlocksB b bs = true.
+Admitted.
+
+Lemma phinodes_placement_wf_fdef: forall (M M':module) (f':fdef)
+  (HeqM: M = module_intro los nts (Ps1 ++ product_fdef (PI_f pinfo) :: Ps2))
+  (HeqM': M' = module_intro los nts (Ps1 ++ product_fdef f' :: Ps2))
+  (HeqF': f' = phinodes_placement_f pinfo (PI_f pinfo))
+  f (HwfF: wf_fdef [M] M f) 
+  (Heq: f = PI_f pinfo) (HuniqF: uniqFdef f), 
+  wf_fdef [M'] M' (phinodes_placement_f pinfo (PI_f pinfo)).
+Proof.
+  intros. subst. assert (HwfF':=HwfF).
+  inv HwfF'.
+  match goal with
+  | Hentry : getEntryBlock _ = _,
+    HuniqF : uniqFdef _,
+    Hnpred : hasNonePredecessor _ _ = _,
+    HwfBs : wf_blocks _ _ _ _ |- _ =>
+     eapply (@TransCFG.pres_getEntryBlock (PhiPlacement pinfo)) 
+       in Hentry; eauto;
+     eapply (@TransCFG.pres_hasNonePredecessor (PhiPlacement pinfo)) 
+       in Hnpred; eauto
+  end.
+  eapply wf_fdef_intro; eauto 2.
+    clear. 
+    apply productInSystemModuleB_intro.
+      simpl. unfold is_true. apply InProductsB_middle.
+
+      unfold moduleInSystem. simpl. apply orb_true_intro. 
+      left. apply moduleEqB_refl.
+       
+    match goal with
+    | H4: wf_fheader _ _ _ |- _ => clear - H4; inv H4
+    end.
+    econstructor; eauto.
+      intros t0 Hint0.
+      apply H0 in Hint0.
+      eapply wf_typ_independent; eauto.
+
+    match goal with
+    | H2: fdef_intro _ _ = PI_f _,
+      H9: wf_blocks _ _ _ _ |- _ =>
+      rewrite H2 in H9;
+      eapply phinodes_placement_wf_blocks in H9; try solve [
+        eauto |
+        rewrite <- H2; fold_PhiPlacement_tac |
+        rewrite <- H2 in HuniqF; eapply uniqF__uniqBlocksLocs; eauto |
+        rewrite <- H2; simpl; intros; apply In_InBlocksB; auto
+      ]
+    end.
+Qed.
+    
+End PresWF.
 
 Lemma phinodes_placement_wfS: forall rd f Ps1 Ps2 los nts pid ty al
   num l0 ps0 cs0 tmn0 dones (Hreach: ret rd = reachablity_analysis f)
@@ -41,13 +511,23 @@ Lemma phinodes_placement_wfS: forall rd f Ps1 Ps2 los nts pid ty al
   wf_system 
     [module_intro los nts
       (Ps1 ++
-       product_fdef (phinodes_placement f rd pid ty al (successors f)
-                    (make_predecessors (successors f))) :: Ps2)].
+       product_fdef (phinodes_placement rd pid ty al (successors f)
+                    (make_predecessors (successors f)) f) :: Ps2)].
 Proof.
   intros.
+  eapply find_promotable_alloca__WF_PhiInfo in Hfind; eauto.
   eapply TopWFS.trans_wfS with (f:=f) in HwfS; intros;
-    eauto using phinodes_placement_wf_fdef, phinodes_placement_uniqFdef,
-                phinodes_placement_fheaderOfFdef.
+    eauto using phinodes_placement_fheaderOfFdef.
+    match goal with
+    | _: WF_PhiInfo ?pinfo0 |- _ =>
+      eapply phinodes_placement_wf_fdef with (pinfo:=pinfo0) in HwfF; eauto
+    end.
+       rewrite <- phinodes_placement_f_spec1 in HwfF; auto.
+
+       apply wf_single_system__wf_uniq_fdef in HwfS.
+       destruct HwfS; auto.
+
+    eapply phinodes_placement__uniqFdef in Hfind; eauto.
 Qed.
 
 Lemma phinodes_placement_wfPI: forall rd f Ps1 Ps2 los nts pid ty al
@@ -58,8 +538,8 @@ Lemma phinodes_placement_wfPI: forall rd f Ps1 Ps2 los nts pid ty al
      wf_system 
        [module_intro los nts (Ps1 ++ product_fdef f :: Ps2)]),
   WF_PhiInfo {|
-    PI_f := phinodes_placement f rd pid ty al (successors f)
-              (make_predecessors (successors f));
+    PI_f := phinodes_placement rd pid ty al (successors f)
+              (make_predecessors (successors f)) f;
     PI_rd := rd;
     PI_id := pid;
     PI_typ := ty;
@@ -67,17 +547,4 @@ Lemma phinodes_placement_wfPI: forall rd f Ps1 Ps2 los nts pid ty al
     PI_align := al |}.
 Admitted. (* WF prev *)
 
-Lemma phinodes_placement_reachablity_analysis: forall f rd pid ty al,
-  reachablity_analysis f =
-  reachablity_analysis
-     (phinodes_placement f rd pid ty al (successors f)
-        (make_predecessors (successors f))).
-Admitted. (* WF prev *)
-
-Lemma phinodes_placement_reachablity_successors: forall f rd pid ty al,
-  successors f =
-  successors
-    (phinodes_placement f rd pid ty al (successors f)
-       (make_predecessors (successors f))).
-Admitted. (* WF prev *)
 
