src3.0/Transforms/top_wfS.v
@@ -107,103 +107,10 @@ Qed.
 
 Module TopWFS.
 
-Section SubstFdef.
+Section Uniqness.
 
 Variable (f f':fdef).
 Hypothesis (Heq_fheader: fheaderOfFdef f = fheaderOfFdef f').
-
-(* This lemma is provable. But it shows a bug in the typing. 
-   The wf_const_gid rule does not look up types of functions!!
-
-   The second issue is that in all the rules, module is completely 
-   independent. When looking-up gid, wf_const_gid rule searches it from 
-   the entire system directly. We should search from the current module,
-   and then, for external definitions, we should go find other modules
-   in the system. In the case, the system contains only one module (which
-   is the assumption of the current design), this is not an issue. But,
-   we may want to fix it.
-
-   The third point is that we should simplify typing rules to carry a ctx
-   that only takes the signatures of products, rather than the entire 
-   definitions, then the following lemma is trivial!
-*)
-Lemma subst_fdef_preserves_wf_the_prod: forall M M' los nts Ps1 Ps2 Ms1 Ms2
-  prod (HeqM: M = module_intro los nts (Ps1 ++ product_fdef f :: Ps2))
-  (HeqM': M' = module_intro los nts (Ps1 ++ product_fdef f' :: Ps2))
-  (HwfPs: wf_prod (Ms1 ++ M :: Ms2) M prod),
-  wf_prod (Ms1 ++ M' :: Ms2) M' prod.
-Admitted. (* need to fix typing *)
-
-Lemma subst_fdef_preserves_wf_other_prod: forall M M' los nts Ps1 Ps2 Ms1 
-  Ms2 prod (HeqM: M = module_intro los nts (Ps1 ++ product_fdef f :: Ps2))
-  (HeqM': M' = module_intro los nts (Ps1 ++ product_fdef f' :: Ps2))
-  md (HwfPs: wf_prod (Ms1 ++ M :: Ms2) md prod) (Hin: In md Ms1 \/ In md Ms2),
-  wf_prod (Ms1 ++ M' :: Ms2) md prod.
-Admitted. (* need to fix typing *)
-
-Lemma subst_fdef_in_ctx_preserves_wf_the_fdef: forall M M' los nts Ps2 Ms1 
-  Ms2 Ps1
-  (HeqM: M = module_intro los nts (Ps1 ++ product_fdef f :: Ps2))
-  (HeqM': M' = module_intro los nts (Ps1 ++ product_fdef f' :: Ps2)) f0
-  (HwfF: wf_fdef (Ms1 ++ M :: Ms2) M f0),
-  wf_fdef (Ms1 ++ M' :: Ms2) M' f0.
-Proof.
-  intros.
-  apply wf_prod_function_def in HwfF; try constructor.
-  eapply subst_fdef_preserves_wf_the_prod in HwfF; eauto using in_middle.
-  inv HwfF; auto.
-Qed.
-
-Lemma subst_fdef_preserves_wf_the_module: forall los nts Ps2 
-  Ms1 Ms2 Ps1 S S' M M'
-  (HeqM: M = module_intro los nts (Ps1 ++ product_fdef f :: Ps2))
-  (HeqM': M' = module_intro los nts (Ps1 ++ product_fdef f' :: Ps2))
-  (HeqS: S = Ms1 ++ M :: Ms2) (HeqS': S' = Ms1 ++ M' :: Ms2) 
-  (Hwff': wf_fdef S' M' f') (HwfS : wf_module S M),
-  wf_module S' M'.
-Proof.
-  intros. subst.
-  inv HwfS.
-  constructor.
-    eapply wf_namedts_independent; eauto.
-
-    solve_in_list.
-
-    apply wf_prods_intro.
-      intros.
-
-      destruct_in Hin.
-        eapply wf_prods_elim with (prod:=prod) in H5; eauto.
-          eapply subst_fdef_preserves_wf_the_prod; eauto. 
-          xsolve_in_list.
-      destruct_in Hin.
-        constructor; auto. constructor.
-
-        eapply wf_prods_elim with (prod:=prod) in H5; eauto.
-          eapply subst_fdef_preserves_wf_the_prod; eauto.
-          xsolve_in_list.
-Qed.
-
-Lemma subst_fdef_preserves_wf_other_module: forall los nts Ps2 
-  Ms1 Ms2 Ps1 S S' M M'
-  (HeqM: M = module_intro los nts (Ps1 ++ product_fdef f :: Ps2))
-  (HeqM': M' = module_intro los nts (Ps1 ++ product_fdef f' :: Ps2))
-  (HeqS: S = Ms1 ++ M :: Ms2) (HeqS': S' = Ms1 ++ M' :: Ms2) md
-  (Hin: In md Ms1 \/ In md Ms2) (HwfS : wf_module S md), 
-  wf_module S' md.
-Proof.
-  intros. subst.
-  inv HwfS.
-  constructor.
-    eapply wf_namedts_independent; eauto.
-
-    destruct Hin as [Hin | Hin]; xsolve_in_list.
-
-    apply wf_prods_intro.
-      intros.
-      eapply wf_prods_elim with (prod:=prod) in H1; eauto.
-        eapply subst_fdef_preserves_wf_other_prod; eauto. 
-Qed.
 
 Lemma subst_fdef_preserves_uniqProducts: forall Ps2 (Huniqf': uniqFdef f') Ps1 
   (HuniqPs: uniqProducts (Ps1 ++ product_fdef f :: Ps2)),
@@ -252,12 +159,103 @@ Proof.
   eapply uniqModules_elim in HuniqS; eauto using in_middle. 
 Qed.  
 
+End Uniqness.
+
+Section SubstFdefWF.
+
+Variable (f f':fdef).
+Hypothesis (Heq_fheader: fheaderOfFdef f = fheaderOfFdef f').
+
+(* This lemma is provable. But it shows a bug in the typing. 
+   The wf_const_gid rule does not look up types of functions!!
+
+   The second issue is that in all the rules, module is completely 
+   independent. When looking-up gid, wf_const_gid rule searches it from 
+   the entire system directly. We should search from the current module,
+   and then, for external definitions, we should go find other modules
+   in the system. In the case, the system contains only one module (which
+   is the assumption of the current design), this is not an issue. But,
+   we may want to fix it.
+
+   The third point is that we should simplify typing rules to carry a ctx
+   that only takes the signatures of products, rather than the entire 
+   definitions, then the following lemma is trivial!
+*)
+Lemma subst_fdef_preserves_wf_the_prod: forall M M' los nts Ps1 Ps2 Ms1 
+  Ms2 prod (HeqM: M = module_intro los nts (Ps1 ++ product_fdef f :: Ps2))
+  (HeqM': M' = module_intro los nts (Ps1 ++ product_fdef f' :: Ps2))
+  (HwfPs: wf_prod (Ms1 ++ M :: Ms2) M prod) 
+  (Hin: In prod Ps1 \/ In prod Ps2),
+  wf_prod (Ms1 ++ M' :: Ms2) M' prod.
+Admitted. (* need to fix typing *)
+
+Lemma subst_fdef_preserves_wf_other_prod: forall M M' los nts Ps1 Ps2 Ms1 
+  Ms2 prod (HeqM: M = module_intro los nts (Ps1 ++ product_fdef f :: Ps2))
+  (HeqM': M' = module_intro los nts (Ps1 ++ product_fdef f' :: Ps2))
+  md (HwfPs: wf_prod (Ms1 ++ M :: Ms2) md prod) 
+  (Hin: In md Ms1 \/ In md Ms2),
+  wf_prod (Ms1 ++ M' :: Ms2) md prod.
+Admitted. (* need to fix typing, See subst_fdef_preserves_wf_the_prod *)
+
+Lemma subst_fdef_preserves_wf_other_module: forall los nts Ps2 
+  Ms1 Ms2 Ps1 S S' M M'
+  (HeqM: M = module_intro los nts (Ps1 ++ product_fdef f :: Ps2))
+  (HeqM': M' = module_intro los nts (Ps1 ++ product_fdef f' :: Ps2))
+  (HeqS: S = Ms1 ++ M :: Ms2) (HeqS': S' = Ms1 ++ M' :: Ms2) md
+  (Hin: In md Ms1 \/ In md Ms2) (HwfS : wf_module S md), 
+  wf_module S' md.
+Proof.
+  intros. subst.
+  inv HwfS.
+  constructor.
+    eapply wf_namedts_independent; eauto.
+
+    destruct Hin as [Hin | Hin]; xsolve_in_list.
+
+    apply wf_prods_intro.
+      intros.
+      eapply wf_prods_elim with (prod:=prod) in H1; eauto.
+        eapply subst_fdef_preserves_wf_other_prod; eauto. 
+Qed.
+
+Lemma subst_fdef_preserves_wf_the_module: forall los nts Ps2 
+  Ms1 Ms2 Ps1 S S' M M'
+  (HeqM: M = module_intro los nts (Ps1 ++ product_fdef f :: Ps2))
+  (HeqM': M' = module_intro los nts (Ps1 ++ product_fdef f' :: Ps2))
+  (HeqS: S = Ms1 ++ M :: Ms2) (HeqS': S' = Ms1 ++ M' :: Ms2) 
+  (HwfF': wf_fdef (Ms1 ++ M' :: Ms2) M' f') (HwfS : wf_module S M),
+  wf_module S' M'.
+Proof.
+  intros. subst.
+  inv HwfS.
+  constructor.
+    eapply wf_namedts_independent; eauto.
+
+    solve_in_list.
+
+    apply wf_prods_intro.
+      intros.
+
+      destruct_in Hin.
+        eapply wf_prods_elim with (prod:=prod) in H5; eauto.
+          eapply subst_fdef_preserves_wf_the_prod; eauto. 
+          xsolve_in_list.
+      destruct_in Hin.
+        constructor; auto.
+          constructor.
+
+        eapply wf_prods_elim with (prod:=prod) in H5; eauto.
+          eapply subst_fdef_preserves_wf_the_prod; eauto.
+          xsolve_in_list.
+Qed.
+
 Lemma subst_fdef_preserves_wf_system: forall los nts Ps2 
   Ms1 Ms2 Ps1 S S' M M'
   (HeqM: M = module_intro los nts (Ps1 ++ product_fdef f :: Ps2))
   (HeqM': M' = module_intro los nts (Ps1 ++ product_fdef f' :: Ps2))
   (HeqS: S = Ms1 ++ M :: Ms2) (HeqS': S' = Ms1 ++ M' :: Ms2) 
-  (Hwff': wf_fdef S' M' f') (Huniqf': uniqFdef f') (HwfS : wf_system S),
+  (HwfF': wf_fdef (Ms1 ++ M' :: Ms2) M' f') (Huniqf': uniqFdef f') 
+  (HwfS : wf_system S),
   wf_system S'.
 Proof.
   intros.
@@ -282,26 +280,21 @@ Proof.
     eapply subst_fdef_preserves_uniqSystem in H0; eauto.
 Qed.
 
-Lemma subst_fdef_preserves_wf_single_module: forall los nts M Ps1 Ps2
+Lemma subst_fdef_preserves_wf_single_module: forall los nts M M' Ps1 Ps2
   (HeqM: M = module_intro los nts (Ps1 ++ product_fdef f :: Ps2))
-  (HwfF_pres: wf_fdef [M] M f -> wf_fdef [M] M f') 
-  (Huniq_pres: uniqFdef f -> uniqFdef f') (HwfS : wf_system [M]),
-  wf_system [module_intro los nts (Ps1 ++ product_fdef f' :: Ps2)].
+  (HeqM': M' = module_intro los nts (Ps1 ++ product_fdef f' :: Ps2))
+  (HwfF': wf_fdef [M'] M' f') (Huniqf': uniqFdef f') 
+  (HwfS : wf_system [M]), wf_system [M'].
 Proof.
   intros. subst.
-  assert (Hwf:=HwfS).
-  apply wf_single_system__wf_uniq_fdef in Hwf.
-  destruct Hwf as [HwfF HuniqF].
   repeat match goal with
   | |- context [ [?A ] ] => rewrite_env (nil ++ A :: nil)
   | H:context [ [?A ] ] |- _ => rewrite_env (nil ++ A :: nil) in H
   end.
   eapply subst_fdef_preserves_wf_system; eauto.
-    apply HwfF_pres in HwfF.
-    eapply subst_fdef_in_ctx_preserves_wf_the_fdef in HwfF; eauto.
 Qed.
 
-End SubstFdef.
+End SubstFdefWF.
 
 Section TopWFS.
 
@@ -310,8 +303,8 @@ Variable (f f':fdef).
 Hypothesis trans_wf_fdef: forall los nts Ps1 Ps2
   (HwfF: wf_fdef [module_intro los nts (Ps1 ++ product_fdef f :: Ps2)]
            (module_intro los nts (Ps1 ++ product_fdef f :: Ps2)) f),
-  wf_fdef [module_intro los nts (Ps1 ++ product_fdef f :: Ps2)]
-    (module_intro los nts (Ps1 ++ product_fdef f :: Ps2)) f'.
+  wf_fdef [module_intro los nts (Ps1 ++ product_fdef f' :: Ps2)]
+    (module_intro los nts (Ps1 ++ product_fdef f' :: Ps2)) f'.
 
 Hypothesis trans_uniqFdef: forall (Huniq: uniqFdef f), uniqFdef f'.
 
@@ -322,6 +315,9 @@ Lemma trans_wfS: forall Ps1 Ps2 los nts
   wf_system [module_intro los nts (Ps1 ++ product_fdef f' :: Ps2)].
 Proof.
   intros.
+  assert (Hwf:=HwfS).
+  apply wf_single_system__wf_uniq_fdef in Hwf.
+  destruct Hwf as [HwfF HuniqF].
   eapply subst_fdef_preserves_wf_single_module with (f:=f) in HwfS; eauto.
 Qed.
 
@@ -329,3 +325,368 @@ End TopWFS.
 
 End TopWFS.
 
+Definition getBlockTmn (b:block) : terminator :=
+match b with
+| block_intro _ _ _ tmn => tmn
+end.
+
+Definition terminator_match (tmn1 tmn2: terminator) : Prop :=
+match tmn1, tmn2 with
+| insn_return id1 _ _, insn_return id2 _ _ => id1 = id2
+| insn_return_void id1, insn_return_void id2 => id1 = id2
+| insn_br id1 _ l11 l12, insn_br id2 _ l21 l22 => 
+    id1 = id2 /\ l11 = l21 /\ l12 = l22
+| insn_br_uncond id1 l1, insn_br_uncond id2 l2 => id1 = id2 /\ l1 = l2
+| insn_unreachable i1, insn_unreachable i2 => i1 = i2
+| _, _ => False
+end.
+
+Structure Pass := mkPass {
+btrans: block -> block;
+ftrans: fdef -> fdef;
+ftrans_spec: forall fh bs, 
+  ftrans (fdef_intro fh bs) = fdef_intro fh (List.map btrans bs);
+btrans_eq_label: forall b, getBlockLabel b = getBlockLabel (btrans b);
+btrans_eq_tmn: forall b, 
+  terminator_match (getBlockTmn b) (getBlockTmn (btrans b))
+}.
+
+Ltac ftrans_spec_tac :=
+repeat match goal with
+| H: context [?pass.(ftrans) (fdef_intro _ _)] |- _ => 
+  rewrite pass.(ftrans_spec) in H
+| |- context [?pass.(ftrans) (fdef_intro _ _)] => rewrite pass.(ftrans_spec)
+end.
+
+Ltac btrans_eq_label_tac b :=
+let J:=fresh "J" in
+let l1:=fresh "l1" in
+let R:=fresh "R" in
+match goal with
+| pass: Pass |- _ =>
+  assert (J:=pass.(btrans_eq_label) b);
+  remember (btrans pass b) as R;
+  destruct R as [l1 ? ? ?]; destruct b; simpl in *; subst l1
+end.
+
+Ltac terminator_match_tac :=
+match goal with
+| J : terminator_match ?t1 ?t2 |- _ =>
+  destruct t1; destruct t2; simpl in J; tinv J; auto;
+    match goal with
+    | J': ?id1 = _ /\ ?id2 = _ /\ ?id3 = _ |- _ =>
+      destruct J' as [? [? ?]]; subst id1 id2 id3; auto
+    | J': ?id1 = _ /\ ?id2 = _ |- _ =>
+      destruct J' as [? ?]; subst id1 id2; auto
+    | J' : ?id0 = _ |- _ => subst id0; auto
+    end
+end.
+
+Module TransCFG.
+
+Section TransCFG.
+
+Context `{pass: Pass}.
+
+(************** Preserving wellformedness **************************************)
+
+Lemma pres_getEntryBlock : forall f b
+  (Hentry : getEntryBlock f = Some b),
+  getEntryBlock (pass.(ftrans) f) = Some (pass.(btrans) b).
+Proof.
+  intros. destruct f as [fh bs]. ftrans_spec_tac.
+  destruct bs; inv Hentry; auto.
+Qed.
+
+Lemma pres_getEntryBlock_None : forall f
+  (Hentry : getEntryBlock f = None),
+  getEntryBlock (pass.(ftrans) f) = None.
+Proof.
+  intros. destruct f as [fh bs]. ftrans_spec_tac.
+  destruct bs; inv Hentry; auto.
+Qed.
+
+Lemma pres_genBlockUseDef_block : forall b ud,
+  genBlockUseDef_block b ud =
+  genBlockUseDef_block (pass.(btrans) b) ud.
+Proof.
+  intros.
+  assert (J:=pass.(btrans_eq_tmn) b).
+  btrans_eq_label_tac b.
+  terminator_match_tac.
+Qed.
+
+Lemma pres_genBlockUseDef_blocks : forall bs ud,
+  genBlockUseDef_blocks bs ud =
+  genBlockUseDef_blocks (List.map pass.(btrans) bs) ud.
+Proof.
+  induction bs; simpl; intros; auto.
+    rewrite <- IHbs.
+    rewrite <- pres_genBlockUseDef_block; auto.
+Qed.
+
+Lemma pres_hasNonePredecessor : forall f b
+  (Hnpred : hasNonePredecessor b (genBlockUseDef_fdef f) = true),
+  hasNonePredecessor (pass.(btrans) b)
+    (genBlockUseDef_fdef (pass.(ftrans) f)) = true.
+Proof.
+  unfold hasNonePredecessor. unfold predOfBlock.
+  intros. destruct f as [fh bs]. ftrans_spec_tac. simpl.
+  rewrite <- pres_genBlockUseDef_blocks.
+  rewrite <- pass.(btrans_eq_label). auto.
+Qed.
+
+Lemma pres_InBlocksLabels : forall l0 (bs : blocks)
+  (Hin : In l0 (getBlocksLabels (List.map pass.(btrans) bs))),
+  In l0 (getBlocksLabels bs).
+Proof.
+  induction bs as [|b bs]; simpl; auto.
+    btrans_eq_label_tac b.
+    intro Hin.
+    destruct Hin as [Hin | Hin]; auto.
+Qed.
+
+Lemma pres_uniqBlocksLabels : forall (bs : blocks)
+  (HuniqBs : NoDup (getBlocksLabels bs)),
+  NoDup (getBlocksLabels (List.map pass.(btrans) bs)).
+Proof.
+  induction bs as [|b bs]; simpl; intros; auto.
+    btrans_eq_label_tac b.
+    inv HuniqBs.
+    apply NoDup_cons; eauto using pres_InBlocksLabels.
+Qed.
+
+Lemma pres_blockInFdefB : forall f b
+  (Hin : blockInFdefB b f = true),
+  blockInFdefB (pass.(btrans) b) (pass.(ftrans) f) = true.
+Proof.
+  intros. destruct f as [fh bs]. ftrans_spec_tac. simpl.
+  apply InBlocksB_map; auto.
+Qed.
+
+Hint Resolve pres_blockInFdefB: ssa_trans.
+
+Lemma pres_successors_blocks : forall bs,
+  successors_blocks bs = successors_blocks (List.map pass.(btrans) bs).
+Proof.
+  induction bs as [|b bs]; simpl; auto.
+    assert (J:=pass.(btrans_eq_tmn) b).
+    btrans_eq_label_tac b. 
+    rewrite IHbs.
+    terminator_match_tac.
+Qed.
+
+Hint Resolve pres_successors_blocks: ssa_trans.
+
+Lemma pres_successors : forall f,
+  successors f = successors (pass.(ftrans) f).
+Proof.
+  intros. destruct f. ftrans_spec_tac. simpl. auto with ssa_trans.
+Qed.
+
+Lemma pres_bound_blocks : forall bs,
+  bound_blocks bs = bound_blocks (List.map pass.(btrans) bs).
+Proof.
+  induction bs as [|a bs]; simpl; auto.
+    btrans_eq_label_tac a. congruence.
+Qed.
+
+Lemma pres_bound_fdef : forall f,
+  bound_fdef f = bound_fdef (pass.(ftrans) f).
+Proof.
+  destruct f as [fh bs]. ftrans_spec_tac. simpl.
+  apply pres_bound_blocks.
+Qed.
+
+Lemma pres_vertexes_fdef: forall f,
+  vertexes_fdef f = vertexes_fdef (pass.(ftrans) f).
+Proof.
+  unfold vertexes_fdef.
+  destruct f.  ftrans_spec_tac. simpl. intros.
+  rewrite <- pres_bound_blocks. auto.
+Qed.
+
+Lemma pres_arcs_fdef: forall f,
+  arcs_fdef f = arcs_fdef (pass.(ftrans) f).
+Proof.
+  unfold arcs_fdef.
+  destruct f.  ftrans_spec_tac. simpl. intros.
+  rewrite <- pres_successors_blocks. auto.
+Qed.
+
+Lemma pres_reachable : forall f,
+  reachable f = reachable (pass.(ftrans) f).
+Proof.
+  intros.
+  unfold reachable.
+  case_eq (getEntryBlock f).
+    intros b Hentry.
+    apply pres_getEntryBlock in Hentry; eauto.
+    rewrite Hentry.
+    btrans_eq_label_tac b.
+    rewrite <- pres_vertexes_fdef.
+    rewrite <- pres_arcs_fdef. auto.
+
+    intro Hentry.
+    apply pres_getEntryBlock_None in Hentry; eauto.
+    rewrite Hentry. auto.
+Qed.
+
+Lemma pres_isReachableFromEntry : forall f b,
+  isReachableFromEntry f b =
+    isReachableFromEntry (pass.(ftrans) f) (pass.(btrans) b).
+Proof.
+  unfold isReachableFromEntry. intros.
+  btrans_eq_label_tac b. 
+  rewrite <- pres_reachable; auto.
+Qed.
+
+Lemma pres_areachable_aux : forall f,
+  areachable_aux f = areachable_aux (pass.(ftrans) f).
+Proof.
+  intros.
+  unfold areachable_aux.
+  case_eq (getEntryBlock f).
+    intros b Hentry.
+    apply pres_getEntryBlock in Hentry; eauto.
+    rewrite Hentry.
+    btrans_eq_label_tac b.
+    rewrite <- pres_successors. auto.
+
+    intro Hentry.
+    apply pres_getEntryBlock_None in Hentry; eauto.
+    rewrite Hentry. auto.
+Qed.
+
+Lemma pres_reachablity_analysis : forall f,
+  reachablity_analysis f = reachablity_analysis (pass.(ftrans) f).
+Proof.
+  intros.
+  unfold reachablity_analysis.
+  case_eq (getEntryBlock f).
+    intros b Hentry.
+    apply pres_getEntryBlock in Hentry; eauto.
+    rewrite Hentry.
+    btrans_eq_label_tac b.
+    rewrite <- pres_bound_fdef.
+    rewrite <- pres_areachable_aux. auto.
+
+    intro Hentry.
+    apply pres_getEntryBlock_None in Hentry; eauto.
+    rewrite Hentry. auto.
+Qed.
+
+Lemma pres_blockStrictDominates : forall f b1 b2,
+  blockStrictDominates f b1 b2 <->
+    blockStrictDominates (pass.(ftrans) f) (pass.(btrans) b1) (pass.(btrans) b2).
+Proof.
+  intros.
+  unfold blockStrictDominates. 
+  btrans_eq_label_tac b1. 
+  btrans_eq_label_tac b2. 
+  unfold dom_analyze. destruct f as [fh bs]. ftrans_spec_tac.
+  rewrite <- pres_successors_blocks.
+  remember (entry_dom bs) as R1.
+  remember (entry_dom (List.map pass.(btrans) bs)) as R2.
+  destruct R1 as [x1 Hx1].
+  destruct R2 as [x2 Hx2].
+  destruct x1 as [x1|].
+  Case "1".
+    destruct x1 as [le1 start1].
+    destruct start1.
+    destruct bs_contents as [|l2' bs_contents]; tinv Hx1.
+    destruct x2 as [x2|].
+    SCase "1.1".
+      destruct x2 as [le2 start2].
+      destruct start2.
+      destruct bs_contents as [|l3 bs_contents]; tinv Hx2.
+      destruct bs as [|b bs]; tinv HeqR1.
+      assert (J:=pass.(btrans_eq_label) b).
+      simpl in *.
+      destruct (btrans pass b). 
+      destruct b. 
+      inv HeqR1. inv HeqR2. simpl in J. subst.
+      eapply blockStrictDominates_iff; eauto.
+      rewrite pres_bound_blocks; auto.
+    SCase "1.2".
+      destruct bs; simpl in *; tinv HeqR1.
+        inv Hx2.
+  Case "2".
+    subst. simpl in *. inv HeqR2. split; intro; auto.
+Qed.
+
+Lemma pres_blockDominates : forall f b1 b2,
+  blockDominates f b1 b2 <->
+    blockDominates (pass.(ftrans) f) (pass.(btrans) b1) (pass.(btrans) b2).
+Proof.
+  intros.
+  unfold blockDominates.
+  btrans_eq_label_tac b1. 
+  btrans_eq_label_tac b2. 
+  unfold dom_analyze. destruct f as [fh bs]. ftrans_spec_tac.
+  rewrite <- pres_successors_blocks.
+  remember (entry_dom bs) as R1.
+  remember (entry_dom (List.map pass.(btrans) bs)) as R2.
+  destruct R1 as [x1 Hx1].
+  destruct R2 as [x2 Hx2].
+  destruct x1 as [x1|].
+  Case "1".
+    destruct x1 as [le1 start1].
+    destruct start1.
+    destruct bs_contents as [|l2' bs_contents]; tinv Hx1.
+    destruct x2 as [x2|].
+    SCase "1.1".
+      destruct x2 as [le2 start2].
+      destruct start2.
+      destruct bs_contents as [|l3 bs_contents]; tinv Hx2.
+      destruct bs as [|b bs]; tinv HeqR1.
+      assert (J:=pass.(btrans_eq_label) b).
+      simpl in *.
+      destruct (btrans pass b). 
+      destruct b. 
+      inv HeqR1. inv HeqR2. simpl in J. subst.
+      eapply blockDominates_iff; eauto.
+      rewrite pres_bound_blocks; auto.
+    SCase "1.2".
+      destruct bs; simpl in *; tinv HeqR1.
+        inv Hx2.
+  Case "2".
+    subst. simpl in *. inv HeqR2. split; intro; auto.
+Qed.
+
+Lemma pres_lookupBlockViaLabelFromBlocks : forall l5 bs b,
+  lookupBlockViaLabelFromBlocks bs l5 = ret b ->
+  lookupBlockViaLabelFromBlocks (List.map pass.(btrans) bs) l5 =
+    ret (pass.(btrans) b).
+Proof.
+  unfold lookupBlockViaLabelFromBlocks.
+  induction bs as [|a]; simpl; intros.
+    congruence.
+
+    btrans_eq_label_tac a. 
+    destruct (@eq_dec atom (EqDec_eq_of_EqDec atom EqDec_atom) l5 l0);
+      subst; inv H; auto.
+      congruence.
+Qed.
+
+Hint Resolve pres_lookupBlockViaLabelFromBlocks : ssa_trans.
+
+Lemma pres_lookupBlockViaLabelFromFdef : forall f l5 b,
+  lookupBlockViaLabelFromFdef f l5 = ret b ->
+  lookupBlockViaLabelFromFdef (pass.(ftrans) f) l5 =
+    ret (pass.(btrans) b).
+Proof.
+  destruct f. ftrans_spec_tac. 
+  intros. apply pres_lookupBlockViaLabelFromBlocks; auto.
+Qed.
+
+Lemma pres_predOfBlock : forall b,
+  predOfBlock b = predOfBlock (pass.(btrans) b).
+Proof.
+  intros.
+  btrans_eq_label_tac b. auto.
+Qed.
+
+End TransCFG.
+
+End TransCFG.
