src3.0/Transforms/dae_wfS.v
@@ -9,7 +9,6 @@ Require Import promotable_props.
 Require Import primitives.
 Require Import palloca_props.
 Require Import memory_props.
-Require Import program_sim.
 Require Import trans_tactic.
 Require Import dae.
 Require Import list_facts.
