src3.0/Transforms/las.v
@@ -12,7 +12,6 @@ Require Import palloca_props.
 Require Import alive_store.
 Require Import id_rhs_val.
 Require Import mem2reg.
-Require Import program_sim.
 Require Import memory_props.
 Require Import trans_tactic.
 Require Import top_sim.
