src3.0/Transforms/phiplacement_bsim_top.v
@@ -387,8 +387,8 @@ Lemma uniq_products_phiplacement_simulation: forall f Ps2 rd pid ty
      (Ps1 ++ product_fdef f :: Ps2)
      (Ps1 ++
       product_fdef
-        (phinodes_placement f rd pid ty al (successors f)
-           (make_predecessors (successors f))) :: Ps2).
+        (phinodes_placement rd pid ty al (successors f)
+           (make_predecessors (successors f)) f) :: Ps2).
 Proof.
   induction Ps1; simpl; intros; subst.
     constructor.
@@ -730,8 +730,8 @@ Lemma phinodes_placement_sim: forall rd f Ps1 Ps2 los nts main VarArgs pid ty al
   program_sim
     [module_intro los nts
       (Ps1 ++
-       product_fdef (phinodes_placement f rd pid ty al (successors f)
-                    (make_predecessors (successors f))) :: Ps2)]
+       product_fdef (phinodes_placement rd pid ty al (successors f)
+                    (make_predecessors (successors f)) f) :: Ps2)]
     [module_intro los nts (Ps1 ++ product_fdef f :: Ps2)]
     main VarArgs.
 Proof.
@@ -745,8 +745,8 @@ Proof.
      [module_intro los nts (Ps1 ++ product_fdef f :: Ps2)]
      [module_intro los nts
         (Ps1 ++
-         product_fdef (phinodes_placement f rd pid ty al (successors f)
-                      (make_predecessors (successors f))) :: Ps2)]) as Hssim.
+         product_fdef (phinodes_placement rd pid ty al (successors f)
+                      (make_predecessors (successors f)) f) :: Ps2)]) as Hssim.
     unfold system_simulation.
     constructor; auto.
     repeat split; auto.
